hax-lib/proof-libs/fstar/core/Core_models.Bundle.fst
@@ -1,7 +1,6 @@
-module Core_models.Option
+module Core_models.Bundle
 #set-options "--fuel 0 --ifuel 1 --z3rlimit 15"
 open FStar.Mul
-open Rust_primitives
 
 type t_Option (v_T: Type0) =
   | Option_Some : v_T -> t_Option v_T
@@ -131,33 +130,6 @@ let impl__map_or_default
     Core_models.Ops.Function.f_call_once #v_F #v_T #FStar.Tactics.Typeclasses.solve f t
   | Option_None  -> Core_models.Default.f_default #v_U #FStar.Tactics.Typeclasses.solve ()
 
-let impl__ok_or (#v_T #v_E: Type0) (self: t_Option v_T) (err: v_E)
-    : Core_models.Result.t_Result v_T v_E =
-  match self <: t_Option v_T with
-  | Option_Some v -> Core_models.Result.Result_Ok v <: Core_models.Result.t_Result v_T v_E
-  | Option_None  -> Core_models.Result.Result_Err err <: Core_models.Result.t_Result v_T v_E
-
-let impl__ok_or_else
-      (#v_T #v_E #v_F: Type0)
-      (#[FStar.Tactics.Typeclasses.tcresolve ()]
-          i0:
-          Core_models.Ops.Function.t_FnOnce v_F Prims.unit)
-      (#_: unit{i0.Core_models.Ops.Function.f_Output == v_E})
-      (self: t_Option v_T)
-      (err: v_F)
-    : Core_models.Result.t_Result v_T v_E =
-  match self <: t_Option v_T with
-  | Option_Some v -> Core_models.Result.Result_Ok v <: Core_models.Result.t_Result v_T v_E
-  | Option_None  ->
-    Core_models.Result.Result_Err
-    (Core_models.Ops.Function.f_call_once #v_F
-        #Prims.unit
-        #FStar.Tactics.Typeclasses.solve
-        err
-        (() <: Prims.unit))
-    <:
-    Core_models.Result.t_Result v_T v_E
-
 let impl__and_then
       (#v_T #v_U #v_F: Type0)
       (#[FStar.Tactics.Typeclasses.tcresolve ()] i0: Core_models.Ops.Function.t_FnOnce v_F v_T)
@@ -198,3 +170,125 @@ let impl__unwrap (#v_T: Type0) (self: t_Option v_T)
   match self <: t_Option v_T with
   | Option_Some v_val -> v_val
   | Option_None  -> Core_models.Panicking.Internal.panic #v_T ()
+
+type t_Result (v_T: Type0) (v_E: Type0) =
+  | Result_Ok : v_T -> t_Result v_T v_E
+  | Result_Err : v_E -> t_Result v_T v_E
+
+let impl__ok_or (#v_T #v_E: Type0) (self: t_Option v_T) (err: v_E) : t_Result v_T v_E =
+  match self <: t_Option v_T with
+  | Option_Some v -> Result_Ok v <: t_Result v_T v_E
+  | Option_None  -> Result_Err err <: t_Result v_T v_E
+
+let impl__ok_or_else
+      (#v_T #v_E #v_F: Type0)
+      (#[FStar.Tactics.Typeclasses.tcresolve ()]
+          i0:
+          Core_models.Ops.Function.t_FnOnce v_F Prims.unit)
+      (#_: unit{i0.Core_models.Ops.Function.f_Output == v_E})
+      (self: t_Option v_T)
+      (err: v_F)
+    : t_Result v_T v_E =
+  match self <: t_Option v_T with
+  | Option_Some v -> Result_Ok v <: t_Result v_T v_E
+  | Option_None  ->
+    Result_Err
+    (Core_models.Ops.Function.f_call_once #v_F
+        #Prims.unit
+        #FStar.Tactics.Typeclasses.solve
+        err
+        (() <: Prims.unit))
+    <:
+    t_Result v_T v_E
+
+let impl__map__from__result
+      (#v_T #v_E #v_U #v_F: Type0)
+      (#[FStar.Tactics.Typeclasses.tcresolve ()] i0: Core_models.Ops.Function.t_FnOnce v_F v_T)
+      (#_: unit{i0.Core_models.Ops.Function.f_Output == v_U})
+      (self: t_Result v_T v_E)
+      (op: v_F)
+    : t_Result v_U v_E =
+  match self <: t_Result v_T v_E with
+  | Result_Ok t ->
+    Result_Ok (Core_models.Ops.Function.f_call_once #v_F #v_T #FStar.Tactics.Typeclasses.solve op t)
+    <:
+    t_Result v_U v_E
+  | Result_Err e -> Result_Err e <: t_Result v_U v_E
+
+let impl__map_or__from__result
+      (#v_T #v_E #v_U #v_F: Type0)
+      (#[FStar.Tactics.Typeclasses.tcresolve ()] i0: Core_models.Ops.Function.t_FnOnce v_F v_T)
+      (#_: unit{i0.Core_models.Ops.Function.f_Output == v_U})
+      (self: t_Result v_T v_E)
+      (v_default: v_U)
+      (f: v_F)
+    : v_U =
+  match self <: t_Result v_T v_E with
+  | Result_Ok t ->
+    Core_models.Ops.Function.f_call_once #v_F #v_T #FStar.Tactics.Typeclasses.solve f t
+  | Result_Err e_e -> v_default
+
+let impl__map_or_else__from__result
+      (#v_T #v_E #v_U #v_D #v_F: Type0)
+      (#[FStar.Tactics.Typeclasses.tcresolve ()] i0: Core_models.Ops.Function.t_FnOnce v_F v_T)
+      (#_: unit{i0.Core_models.Ops.Function.f_Output == v_U})
+      (#[FStar.Tactics.Typeclasses.tcresolve ()] i1: Core_models.Ops.Function.t_FnOnce v_D v_E)
+      (#_: unit{i1.Core_models.Ops.Function.f_Output == v_U})
+      (self: t_Result v_T v_E)
+      (v_default: v_D)
+      (f: v_F)
+    : v_U =
+  match self <: t_Result v_T v_E with
+  | Result_Ok t ->
+    Core_models.Ops.Function.f_call_once #v_F #v_T #FStar.Tactics.Typeclasses.solve f t
+  | Result_Err e ->
+    Core_models.Ops.Function.f_call_once #v_D #v_E #FStar.Tactics.Typeclasses.solve v_default e
+
+let impl__map_err
+      (#v_T #v_E #v_F #v_O: Type0)
+      (#[FStar.Tactics.Typeclasses.tcresolve ()] i0: Core_models.Ops.Function.t_FnOnce v_O v_E)
+      (#_: unit{i0.Core_models.Ops.Function.f_Output == v_F})
+      (self: t_Result v_T v_E)
+      (op: v_O)
+    : t_Result v_T v_F =
+  match self <: t_Result v_T v_E with
+  | Result_Ok t -> Result_Ok t <: t_Result v_T v_F
+  | Result_Err e ->
+    Result_Err
+    (Core_models.Ops.Function.f_call_once #v_O #v_E #FStar.Tactics.Typeclasses.solve op e)
+    <:
+    t_Result v_T v_F
+
+let impl__is_ok (#v_T #v_E: Type0) (self: t_Result v_T v_E) : bool =
+  match self <: t_Result v_T v_E with
+  | Result_Ok _ -> true
+  | _ -> false
+
+let impl__and_then__from__result
+      (#v_T #v_E #v_U #v_F: Type0)
+      (#[FStar.Tactics.Typeclasses.tcresolve ()] i0: Core_models.Ops.Function.t_FnOnce v_F v_T)
+      (#_: unit{i0.Core_models.Ops.Function.f_Output == t_Result v_U v_E})
+      (self: t_Result v_T v_E)
+      (op: v_F)
+    : t_Result v_U v_E =
+  match self <: t_Result v_T v_E with
+  | Result_Ok t ->
+    Core_models.Ops.Function.f_call_once #v_F #v_T #FStar.Tactics.Typeclasses.solve op t
+  | Result_Err e -> Result_Err e <: t_Result v_U v_E
+
+let impl__ok (#v_T #v_E: Type0) (self: t_Result v_T v_E) : t_Option v_T =
+  match self <: t_Result v_T v_E with
+  | Result_Ok x -> Option_Some x <: t_Option v_T
+  | Result_Err _ -> Option_None <: t_Option v_T
+
+let impl__unwrap__from__result (#v_T #v_E: Type0) (self: t_Result v_T v_E)
+    : Prims.Pure v_T (requires impl__is_ok #v_T #v_E self) (fun _ -> Prims.l_True) =
+  match self <: t_Result v_T v_E with
+  | Result_Ok t -> t
+  | Result_Err _ -> Core_models.Panicking.Internal.panic #v_T ()
+
+let impl__expect__from__result (#v_T #v_E: Type0) (self: t_Result v_T v_E) (e_msg: string)
+    : Prims.Pure v_T (requires impl__is_ok #v_T #v_E self) (fun _ -> Prims.l_True) =
+  match self <: t_Result v_T v_E with
+  | Result_Ok t -> t
+  | Result_Err _ -> Core_models.Panicking.Internal.panic #v_T ()
