hax-lib/proof-libs/fstar/core/Core_models.Fmt.fsti
@@ -1,6 +1,7 @@
 module Core_models.Fmt
 #set-options "--fuel 0 --ifuel 1 --z3rlimit 15"
 open FStar.Mul
+open Rust_primitives
 
 type t_Error = | Error : t_Error
 
